pcuic/theories/PCUICConversionInversion.v
@@ -1,0 +1,216 @@
+From Equations Require Import Equations.
+From MetaCoq.PCUIC Require Import PCUICAst.
+From MetaCoq.PCUIC Require Import PCUICAstUtils.
+From MetaCoq.PCUIC Require Import PCUICCumulativity.
+From MetaCoq.PCUIC Require Import PCUICCumulProp.
+From MetaCoq.PCUIC Require Import PCUICEquality.
+From MetaCoq.PCUIC Require Import PCUICNormal.
+From MetaCoq.PCUIC Require Import PCUICReduction.
+From MetaCoq.PCUIC Require Import PCUICTyping.
+From MetaCoq.Template Require Import config.
+From MetaCoq.Template Require Import utils.
+
+Local Set Keyed Unification.
+
+Set Default Goal Selector "!".
+
+Section fixed.
+  Context {cf : checker_flags}.
+  Context (Σ : global_env_ext).
+  Context (wf : ∥wf_ext Σ∥).
+  
+  Definition conv_pb_rel (pb : conv_pb) :=
+    match pb with
+    | Conv => eq_universe
+    | Cumul => leq_universe
+    end.
+  
+  Definition eq_termp_napp leq napp :=
+    eq_term_upto_univ_napp Σ (eq_universe Σ) (conv_pb_rel leq Σ) napp.
+  
+  Notation eq_termp leq := (eq_termp_napp leq 0).
+  
+  Lemma eq_termp_mkApps_inv leq v args v' args' :
+    isApp v = false ->
+    isApp v' = false ->
+    eq_termp leq (mkApps v args) (mkApps v' args') ->
+    eq_termp_napp leq #|args| v v' × All2 (fun x y => eq_term Σ Σ x y) args args'.
+  Proof.
+    intros noapp1 noapp2 eq.
+    now apply eq_term_upto_univ_mkApps_inv in eq as (?&?).
+  Qed.
+  
+  Definition isIndConstructApp (t : term) : bool :=
+    match (decompose_app t).1 with
+    | tInd _ _
+    | tConstruct _ _ _ => true
+    | _ => false
+    end.
+
+  Lemma isIndConstructApp_mkApps hd args :
+    isIndConstructApp (mkApps hd args) = isIndConstructApp hd.
+  Proof.
+    unfold isIndConstructApp.
+    destruct (mkApps_elim hd args).
+    now rewrite !decompose_app_mkApps by easy.
+  Qed.
+
+  Lemma eq_term_upto_univ_napp_nonind Re Rle napp t t' :
+    eq_term_upto_univ_napp Σ Re Rle napp t t' ->
+    isIndConstructApp t = false ->
+    eq_term_upto_univ Σ Re Rle t t'.
+  Proof.
+    intros eq not_ind.
+    generalize 0.
+    intros k.
+    induction eq in k, not_ind |- *; eauto using eq_term_upto_univ_napp.
+    - rewrite (isIndConstructApp_mkApps _ [u]) in not_ind.
+      constructor; auto.
+    - discriminate not_ind.
+    - discriminate not_ind.
+  Qed.
+
+  Lemma whne_red1_isIndConstructApp Γ t t' :
+    whne RedFlags.default Σ Γ t ->
+    red1 Σ Γ t t' ->
+    isIndConstructApp t' = isIndConstructApp t.
+  Proof.
+    apply (whne_red1_ind
+             RedFlags.default Σ Γ
+             (fun t t' => isIndConstructApp t' = isIndConstructApp t)); intros; cbn in *; try easy.
+    - now rewrite !(isIndConstructApp_mkApps _ [v]).
+    - now rewrite (isIndConstructApp_mkApps _ [v]), (isIndConstructApp_mkApps _ [N2]).
+    - now rewrite !isIndConstructApp_mkApps.
+    - now rewrite !isIndConstructApp_mkApps.
+    - now rewrite !isIndConstructApp_mkApps.
+  Qed.
+
+  Lemma whne_red_isIndConstructApp Γ t t' :
+    whne RedFlags.default Σ Γ t ->
+    red Σ Γ t t' ->
+    isIndConstructApp t' = isIndConstructApp t.
+  Proof.
+    intros wh r.
+    induction r in wh |- * using red_rect_n1.
+    - easy.
+    - apply whne_red1_isIndConstructApp in X as ->; eauto.
+      eapply whne_pres; eauto.
+  Qed.
+
+  Lemma conv_cum_alt leq Γ t t' :
+    conv_cum leq Σ Γ t t' <->
+    ∥∑ v v', (red Σ Γ t v × red Σ Γ t' v') × eq_termp leq v v'∥.
+  Proof.
+    assert (forall P Q, (P <~> Q) -> (∥P∥ <-> ∥Q∥)) by
+        (intros P Q H; split; intros [p]; constructor; apply H in p; auto).
+    destruct leq; cbn; apply H; [apply conv_alt_red|apply cumul_alt].
+  Qed.
+
+  Lemma eq_term_eq_termp leq x y :
+    eq_term Σ Σ x y ->
+    eq_termp leq x y.
+  Proof.
+    destruct leq; [easy|].
+    cbn.
+    now apply PCUICCumulProp.eq_term_upto_univ_napp_leq.
+  Qed.
+
+  Lemma conv_cum_mkApps_inv leq Γ hd args hd' args' :
+    conv_cum leq Σ Γ (mkApps hd args) (mkApps hd' args') ->
+    match hd with
+    | tApp _ _
+    | tInd _ _
+    | tConstruct _ _ _ => False
+    | _ => True
+    end ->
+    match hd' with
+    | tApp _ _
+    | tInd _ _
+    | tConstruct _ _ _ => False
+    | _ => True
+    end ->
+    whne RedFlags.default Σ Γ hd ->
+    whne RedFlags.default Σ Γ hd' ->
+    ∥conv_cum leq Σ Γ hd hd' × All2 (conv Σ Γ) args args'∥.
+  Proof.
+    intros conv shape shape' wh wh'.
+    apply conv_cum_alt in conv as [(?&?&(r1&r2)&e)].
+    eapply whne_red_from_mkApps in r1; auto; [|now destruct hd].
+    destruct r1 as [(?&?&->&?&?)].
+    eapply whne_red_from_mkApps in r2; auto; [|now destruct hd'].
+    destruct r2 as [(?&?&->&?&?)].
+    apply eq_termp_mkApps_inv in e as (?&?).
+    2-3: erewrite whne_red_isApp; [| |now eauto]; eauto; try now destruct hd, hd'.
+    constructor.
+    split.
+    - apply conv_cum_alt.
+      constructor.
+      exists x1, x.
+      split; eauto.
+      eapply eq_term_upto_univ_napp_nonind; eauto.
+      erewrite whne_red_isIndConstructApp; [| |now eauto]; eauto.
+      now destruct hd.
+    - clear -a1 a a0.
+      induction a1 in args, args', x2, a, x3, a0, a1 |- *; depelim a; depelim a0; [now constructor|].
+      constructor.
+      + apply conv_alt_red.
+        now exists x, y.
+      + now apply IHa1.
+  Qed.
+  
+  Lemma conv_cum_tCase_inv leq Γ p motive discr brs p' motive' discr' brs' :
+    conv_cum leq Σ Γ (tCase p motive discr brs) (tCase p' motive' discr' brs') ->
+    whnf RedFlags.default Σ Γ (tCase p motive discr brs) ->
+    whnf RedFlags.default Σ Γ (tCase p' motive' discr' brs') ->
+    ∥ p = p' ×
+      Σ;;; Γ |- motive = motive' ×
+      Σ;;; Γ |- discr = discr' ×
+      All2 (fun br br' => br.1 = br'.1 × Σ;;; Γ |- br.2 = br'.2) brs brs'∥.
+  Proof.
+    intros conv whl whr.
+    depelim whl; solve_discr.
+    depelim H; solve_discr; try discriminate.
+    depelim whr; solve_discr.
+    depelim H0; solve_discr; try discriminate.
+    apply conv_cum_alt in conv as [(?&?&(r1&r2)&?)].
+    apply whne_red_from_tCase in r1 as [(?&?&?&->&?&?&?)]; auto.
+    apply whne_red_from_tCase in r2 as [(?&?&?&->&?&?&?)]; auto.
+    depelim e.
+    constructor.
+    split; [easy|].
+    split; [apply conv_alt_red; now exists x1, x|].
+    split; [apply conv_alt_red; now exists x2, x4|].
+    clear -a a0 a1.
+    induction a1 in brs, brs', x3, a, x5, a0, a1 |- *; depelim a; depelim a0; [now constructor|].
+    constructor.
+    + destruct p, p0, r.
+      split; [congruence|].
+      apply conv_alt_red; now exists x.2, y.2.
+    + now apply IHa1.
+  Qed.
+  
+  (* TODO: Remove to a place that actually should be depending on typing *)
+  Lemma conv_cum_red_inv leq Γ t1 t2 t1' t2' :
+    conv_cum leq Σ Γ t1 t2 ->
+    red Σ Γ t1 t1' ->
+    red Σ Γ t2 t2' ->
+    conv_cum leq Σ Γ t1' t2'.
+  Proof.
+    destruct wf.
+    intros cc r1 r2.
+    destruct leq; cbn in *.
+    - destruct cc.
+      constructor.
+      eapply PCUICConversion.conv_red_l_inv; [eauto| |eauto].
+      apply conv_sym.
+      eapply PCUICConversion.conv_red_l_inv; [eauto| |eauto].
+      apply conv_sym.
+      auto.
+    - destruct cc.
+      constructor.
+      eapply PCUICConversion.cumul_red_l_inv; [eauto| |eauto].
+      eapply PCUICConversion.cumul_red_r_inv; [eauto| |eauto].
+      auto.
+  Qed.
+
+End fixed.
