safechecker/theories/PCUICSafeReduce.v
@@ -1659,9 +1659,6 @@ Section Reduce.
       assumption.
   Qed.
               
-  Lemma stack_context_decompose' π π' :
-    stack_context (decompose_stack π).2 = stack_context p.
-
   Theorem reduce_term_complete Γ t h :
     whnf flags Σ Γ (reduce_term Γ t h).
   Proof.
